Extensional, Composition-style mergeable states
Experiment with an "extensional" version of the mergeability relation
between pairs of states, a natural continuation of the current
definition in Composition. Moreover, to keep theorem statements
lightweight and as close to their Composition counterparts (and their
proofs) as possible while we do the portability, remove the option type
from the merge operation (still given as a placeholder) while ensuring
that the operation is only performed when the relation holds.

Intermediate/Recombination.v
@@ -25,6 +25,12 @@ Set Bullet Behavior "Strict Subproofs".
 
 Import Intermediate.
 
+(* RB: NOTE: The current build depends on PS and Composition, both taking a
+   relatively long time to compile, but it may still be desirable to consult
+   them interactively. To speed up the build process, small, tentative additions
+   to those modules can be added here. Note that, in principle, the role of PS
+   will be assimilated by Recombination or become very reduced. *)
+
 Section BehaviorStar.
   Variables p c: program.
 
@@ -131,33 +137,35 @@ Section Recombination.
   Hypothesis Hprog_is_closed  : closed_program (program_link p  c ).
   Hypothesis Hprog_is_closed' : closed_program (program_link p' c').
 
-  Inductive mergeable_states (iface1 iface2 : Program.interface) (s1 s2 : CS.state) : Prop.
+  (* An "extensional" reading of program states a la Composition. *)
+  Inductive mergeable_states (s s'' : CS.state) : Prop :=
+    mergeable_states_intro : forall s0 s0'' t,
+      initial_state (CS.sem (program_link p  c )) s0   ->
+      initial_state (CS.sem (program_link p' c')) s0'' ->
+      Star (CS.sem (program_link p  c )) s0   t s   ->
+      Star (CS.sem (program_link p' c')) s0'' t s'' ->
+      mergeable_states s s''.
 
-  Definition merge_states (s1 s2 : CS.state) : option CS.state :=
-    None.
+  Definition merge_states (s s'' : CS.state) : CS.state :=
+    s.
 
   Theorem initial_states_mergeability s s'' :
     initial_state (CS.sem (program_link p  c )) s   ->
     initial_state (CS.sem (program_link p' c')) s'' ->
-    mergeable_states (prog_interface p) (prog_interface c) s s''.
+    mergeable_states s s''.
   Admitted.
 
   Lemma initial_state_merge_after_linking s s'' :
     initial_state (CS.sem (program_link p  c )) s   ->
     initial_state (CS.sem (program_link p' c')) s'' ->
-  exists s',
-    merge_states s s'' = Some s' /\
-    initial_state (CS.sem (program_link p  c')) s'.
+    initial_state (CS.sem (program_link p  c')) (merge_states s s'').
   Admitted.
 
   Theorem threeway_multisem_star_simulation s1 s1'' t s2 s2'' :
-    mergeable_states (prog_interface p) (prog_interface c) s1 s1'' ->
+    mergeable_states s1 s1'' ->
     Star (CS.sem (program_link p  c )) s1   t s2   ->
     Star (CS.sem (program_link p' c')) s1'' t s2'' ->
-  exists s1' s2',
-    merge_states s1 s1'' = Some s1' /\
-    merge_states s2 s2'' = Some s2' /\
-    Star (CS.sem (program_link p  c')) s1' t s2'.
+    Star (CS.sem (program_link p  c')) (merge_states s1 s1'') t (merge_states s2 s2'').
     (* /\ mergeable_states ip ic s2 s2'' *)
   Admitted.
 
